9/9 pre-meeting update

src/basicmodal/semantics/consistency.lean
@@ -54,52 +54,48 @@ exact mp (mp pl4 (cut (mp pl5 and_commute) (imp_and_imp (mp pl5 L'_ih))))
   (cut iden (cut (imp_and_imp (mp pl6 L'_ih)) (mp pl6 and_commute)))
 end 
 
-lemma nprfalse : ¬ prfK ∅ ⊥ :=
+
+lemma nprfalse (AX : ctx) (hax : ¬ sem_csq AX ⊥) : ¬ prfK AX ⊥ :=
 begin
-have h1 : ¬ sem_csq ∅ ⊥ → ¬ prfK ∅ ⊥, from soundness2 ∅ ⊥,
-apply h1,
-by_contradiction h2,
-rw sem_csq at h2,
-let f : frame := { states := nat,
-  h := ⟨0⟩,
-  rel := λ x y : nat, x = y }, 
-specialize h2 f,
-let v : nat → f.states → Prop := λ n x, true,
-specialize h2 v,
-let x : f.states := 42,
-specialize h2 x,
-apply h2,
-intros y φ h3,
-have h4 : φ ∉ ∅, {exact list.not_mem_nil φ},
-exact absurd h3 h4
+have h1 : ¬ sem_csq AX ⊥ → ¬ prfK AX ⊥, 
+{have h2 : prfK AX ⊥ → sem_csq AX ⊥, from soundness AX ⊥, rw ←not_imp_not at h2, exact h2},
+apply h1, exact hax
 end
 
 
-lemma fin_conj_empty {AX : ctx} {L : list form} :
+lemma fin_conj_empty {AX : ctx} {L : list form} (hax : ¬ sem_csq AX ⊥) :
   L = [] → ¬ prfK AX (fin_conj L ⊃ ⊥) :=
 begin
 intro h1, subst h1, rw fin_conj, simp at *,
 have h1 : prfK AX (¬⊥), from iden,
 simp at *, by_contradiction h2,
 have h3 : prfK AX ⊥, from mp h2 h1,
-have h4 : ¬ prfK AX ⊥, sorry,
+have h4 : ¬ prfK AX ⊥, from nprfalse AX hax,
 exact absurd h3 h4
 end 
+
+lemma listempty {Γ : ctx} {L : list form} :
+  (∀ φ ∈ L, φ ∈ Γ) → Γ = ∅ → L = [] := 
+begin
+intros h1 h2,
+by_contradiction h3,
+have h4 : L ≠ [] → 0 < L.length, from list.length_pos_of_ne_nil,
+specialize h4 h3,
+have h5 : 0 < L.length → ∃ a, a ∈ L, from list.exists_mem_of_length_pos,
+specialize h5 h4,
+cases h5 with φ h5, specialize h1 φ h5,
+have h6 : Γ = ∅ → ∀ φ, φ ∉ Γ, from set.eq_empty_iff_forall_not_mem.mp,
+specialize h6 h2, specialize h6 φ, exact absurd h1 h6
+end
+
 
 -- consistency for a finite set of formulas L
 def fin_ax_consist (AX : ctx) (L : list form) := ¬ prfK AX (fin_conj L ⊃ ⊥)
 
 
 -- consistency for an arbitrary set of formulas Γ
-def ax_consist (AX Γ : ctx) := 
+def ax_consist (AX Γ : ctx) :=
   ∀ L : list form, (∀ ψ ∈ L, ψ ∈ Γ) → fin_ax_consist AX L
- 
--- -- consistency for an arbitrary set of formulas Γ
--- def ax_consist' (AX : ctx) : ctx → list form → Prop
--- | Γ [] := fin_ax_consist AX []
--- | Γ L := (∀ ψ ∈ L, ψ ∈ Γ) → fin_ax_consist AX L
-
--- #check ax_consist'
 
 
 -- Γ is maximally ax-consistent
@@ -182,18 +178,9 @@ cases h2 with h2l h2r, rw max_ax_consist at h1,
 cases h1 with h1l h1r, clear h, 
 have h2 := h1r (Γ ∪ φ), simp at h2, have h3 := h1r (Γ ∪ ¬φ),
 simp at h3, have h4 : ¬ax_consist AX (Γ ∪ ¬φ), 
-{simp at *, apply h3, rw set.ssubset_iff_subset_not_subset, 
-split, 
-rw set.subset_def, intros x h4, exact or.inr h4,
-rw set.not_subset, existsi (¬φ : form), simp, split, 
-apply set.mem_union_left, rw set.mem_def, exact h2r},
+{apply h3, from set.ssubset_insert h2r},
 have h5 : ¬ax_consist AX (Γ ∪ φ), 
-{simp at *, apply h2,
-rw set.ssubset_iff_subset_not_subset, 
-split, 
-rw set.subset_def, intros x h4, exact or.inr h4,
-rw set.not_subset, existsi (φ : form), split, 
-apply set.mem_union_left, rw set.mem_def, exact h2l}, 
+{simp at *, apply h2, from set.ssubset_insert h2l}, 
 clear h2 h3, simp at *, have h6 := five AX Γ φ _, have h7 := five AX Γ (¬φ) _, 
 cases h6 with L' h6, cases h7 with L h7, dsimp at *, cases h6 with h6l h6r,
 cases h7 with h7l h7r,
@@ -211,14 +198,16 @@ specialize h1l h13, exact absurd h12 h1l,
 exact h4,
 exact h5},
 {intro h1, dsimp at h1, rw max_ax_consist, split, exact h,
-intro Γ', intro h2, rw set.ssubset_iff_subset_not_subset at h2, cases h2,
-rw set.not_subset at h2_right,
-apply (exists.elim h2_right), simp, intros ψ h3 h4,
-specialize h1 ψ, cases h1, apply absurd h1 h4,
-have h5 : (¬ψ) ∈ Γ', from set.mem_of_subset_of_mem h2_left h1,
+intro Γ', intro h2,
+have h3 : Γ ⊆ Γ' ∧ ¬ Γ' ⊆ Γ, from h2,
+cases h3,
+rw set.not_subset at h3_right,
+apply (exists.elim h3_right), simp, intros ψ h4 h5,
+specialize h1 ψ, cases h1, apply absurd h1 h5,
+have h6 : (¬ψ) ∈ Γ', from set.mem_of_subset_of_mem h3_left h1,
 rw ax_consist, rw not_forall, existsi ([ψ,¬ψ] : list form),
-simp, split, intros φ h6, cases h6, subst h6, exact h3, 
-subst h6, exact h5, rw fin_ax_consist, rw not_not,
+simp, split, intros φ h7, cases h7, subst h7, exact h4, 
+subst h7, exact h6, rw fin_ax_consist, rw not_not,
 exact fin_conj_simp ψ}
 end
 
@@ -233,7 +222,7 @@ split,
 intros Γ' h2 h3, rw set.subset.antisymm_iff, split, exact h3,
 by_contradiction h4, rw max_ax_consist at h1, cases h1, 
 have h5 := and.intro h3 h4, 
-have h6 : Γ ⊂ Γ', from set.ssubset_iff_subset_not_subset.mpr h5,
+have h6 : Γ ⊂ Γ', from h5,
 specialize h1_right Γ' h6, exact h1_right h2}, 
 intro h1, cases h1, rw max_ax_consist, split, exact h1_left,
 intros Γ' h2, by_contradiction h3, specialize h1_right Γ' h3,
@@ -242,29 +231,90 @@ end
 
 open zorn
 
+
+--Lemma: if c is a chain of sets, L is a list of elements such that 
+--every element in L is in Union(c), then there is an element s in c such that every element of L is in s.
+-- by induction on L.
+-- S := collection of max cons sets
+-- m := Γ'
+
+lemma lindenhelper (c : set ctx) (h : chain (⊆) c) (L : list form) :
+(∀ φ : form, φ ∈ L → φ ∈ ⋃₀(c)) → ∃ ub ∈ c, ∀ ψ : form, ψ ∈ L → ψ ∈ ub :=
+begin
+intro h, sorry
+end
+
 lemma lindenbaum (AX Γ : ctx) (hax : ax_consist AX Γ) : ∃ Γ', max_ax_consist AX Γ' ∧ Γ ⊆ Γ' :=
 begin
 let S := { Γ'' | Γ'' ⊇ Γ ∧ ax_consist AX Γ''},
-have h : ∀c ⊆ S, chain (⊆) c → ∃ub ∈ S, ∀ s ∈ c, s ⊆ ub, {sorry},
+have h : ∀ c ⊆ S, chain (⊆) c → ∃ub ∈ S, ∀ s ∈ c, s ⊆ ub, 
+{intros c h1 h2, 
+have h1 := lindenhelper c h2,
+sorry},
 cases zorn_subset S h with Γ' h1, cases h1 with h1 h2,
 use Γ', split, rw max_equiv, split, apply h1.2, 
 intros m h3 h4, symmetry, apply h2 m, split, apply set.subset.trans h1.1 h4,
 exact h3, exact h4, apply h1.1
 end
 
---Lemma: if c is a chain of sets, L is a list of elements such that 
---every element in L is in Union(c), then there is an element S in C such that every element of L is in S.
--- by induction on L.
--- S := collection of max cons sets
--- m := Γ'
-
 
 
 -- Corollary 8
-lemma max_ax_exists (AX : ctx) : ∃ Γ : ctx, max_ax_consist AX Γ :=
+lemma max_ax_exists (AX : ctx) (hax : ¬ sem_csq AX ⊥) : ∃ Γ : ctx, max_ax_consist AX Γ :=
 begin
-have hax : ax_consist AX ∅, 
-{rw ax_consist, intros L h1, rw fin_ax_consist, by_contradiction h2, sorry},
-have h1 : ∃ Γ, max_ax_consist AX Γ ∧ ∅ ⊆ Γ, from lindenbaum AX ∅ hax, 
-cases h1 with Γ h1, cases h1 with h1 h2, existsi (Γ : ctx), apply h1
+have h1 : ax_consist AX ∅,
+{rw ax_consist, intro L, intro h2, rw fin_ax_consist, 
+have h3 := listempty h2, have this : ∅ = ∅, refl, 
+specialize h3 this, subst h3, by_contradiction h4, 
+have h5 := mp dne, apply nprfalse AX hax, exact h5 h4},
+have h2 : ∃ Γ, max_ax_consist AX Γ ∧ ∅ ⊆ Γ, from lindenbaum AX ∅ h1, 
+cases h2 with Γ h2, cases h2 with h2 h3, existsi (Γ : ctx), apply h2
 end
+
+
+
+
+
+
+
+namespace canonical
+
+def canonical (AX : ctx) (hax : ¬ sem_csq AX ⊥) : frame := 
+{ 
+  states := {x : ctx // max_ax_consist AX x},
+  h := begin have h1 := max_ax_exists AX hax, choose Γ h1 using h1, exact ⟨⟨Γ, h1⟩⟩ end,
+  rel := λ x y, ∀ φ : form, □φ ∈ x → φ ∈ y
+}
+#check canonical
+
+def val_canonical (AX : ctx) (hax : ¬ sem_csq AX ⊥) : nat → (canonical AX hax).states → Prop :=
+λ n, λ x : (canonical AX hax).states, (p n) ∈ x
+
+def form_hat (AX : ctx) (hax : ¬ sem_csq AX ⊥) : form → (canonical AX hax).states → Prop :=
+λ φ, λ x : (canonical AX hax).states, φ ∈ x
+
+lemma existence (AX : ctx) (hax : ¬ sem_csq AX ⊥) (Γ : (canonical AX hax).states) :
+  ∀ φ, ◇φ ∈ Γ → ∃ Δ : (canonical AX hax).states, φ ∈ Δ ∧ (canonical AX hax).rel Γ Δ := sorry
+
+lemma truth (AX : ctx) (hax : ¬ sem_csq AX ⊥) 
+  (v : nat → (canonical AX hax).states → Prop) (x : (canonical AX hax).states) : 
+  ∀ φ, forces (canonical AX hax) v x φ = form_hat AX hax φ x := sorry
+
+theorem completeness (K : ctx) (φ : form) : sem_csq K φ → prfK K φ :=
+begin
+rw ←not_imp_not, intro h1,
+have h2 : ax_consist K {¬φ}, 
+{simp at *, rw ax_consist, intros L h2, rw fin_ax_consist,
+have h3 : L = [¬φ], sorry,
+subst h3, simp at *, rw fin_conj, rw fin_conj, simp at *, 
+have h4 : prfK K ((¬(¬φ)) ⊃ (¬(¬φ)&¬⊥)), sorry,
+have h6 : prfK K (φ ⊃ (¬(¬φ)&¬⊥)), simp at *,
+sorry
+},
+have h3 : ∃ Γ', max_ax_consist K Γ' ∧ {¬φ} ⊆ Γ', from lindenbaum K {¬φ} h2,
+simp at *,
+cases h3 with Γ' h3, cases h3 with h3 h4, sorry
+end
+
+
+end canonical
